thys/BTree/Array_SBlit.thy
@@ -2,6 +2,26 @@ theory Array_SBlit
   imports "Separation_Logic_Imperative_HOL.Array_Blit"
 begin
 
+(* Resolves TODO by Peter Lammich *)
+(* OCaml handles the case of len=0 correctly (i.e.
+as specified by the Hoare Triple in Array_Blit
+not generating an exception if si+len \<le> array length and such) *) 
+code_printing code_module "array_blit" \<rightharpoonup> (OCaml)
+  \<open>
+   let array_blit src si dst di len = (
+      if src=dst then
+         raise (Invalid_argument "array_blit: Same arrays")
+      else
+        Array.blit src (Z.to_int si) dst (Z.to_int di) (Z.to_int len)
+    )
+\<close>
+
+code_printing constant blit' \<rightharpoonup>
+ (OCaml) "(fun () -> /array'_blit _ _ _ _ _)"
+
+
+export_code blit checking OCaml
+
 section "Same array Blit"
 
 text "The standard framework already provides a function to copy array
@@ -117,7 +137,6 @@ next
 
   have[simp]: "take len (drop si (lsrc[di + len := lsrc ! (si + len)]))
         = take len (drop si lsrc)"
-    sledgehammer
     by (metis Suc.prems(2) ab_semigroup_add_class.add.commute add_le_cancel_right take_drop take_update_cancel)
   have [simp]: "drop (di + len) (lsrc[di + len := lsrc ! (si + len)])
          = lsrc ! (si+len) # drop (Suc di + len) lsrc"
@@ -173,8 +192,10 @@ thm safe_sblit_rule
 subsection "Code Generator Setup"
 
 text "Note that the requirement for correctness
-      is even weaker here than in SML.
-      We therefore manually handle the case where length is 0 (in which case nothing happens at all)."
+      is even weaker here than in SML/OCaml.
+      In particular, if the length of the slice to copy is equal to 0,
+      we will never throw an exception.
+      We therefore manually handle this case, where nothing happens at all."
 
 code_printing code_module "array_sblit" \<rightharpoonup> (SML)
   \<open>
@@ -184,6 +205,15 @@ code_printing code_module "array_sblit" \<rightharpoonup> (SML)
           di = IntInf.toInt di,
           src = ArraySlice.slice (src,IntInf.toInt si,SOME (IntInf.toInt len)),
           dst = src}
+      else ()
+    )
+\<close>
+
+code_printing code_module "array_sblit" \<rightharpoonup> (OCaml)
+  \<open>
+   let array_sblit src si di len = (
+      if len > Z.zero then
+        (Array.blit src (Z.to_int si) src (Z.to_int di) (Z.to_int len))
       else ()
     )
 \<close>
@@ -198,7 +228,7 @@ lemma [code]:
       = safe_sblit' src (integer_of_nat si) (integer_of_nat di) 
           (integer_of_nat len)" by (simp add: safe_sblit'_def)
 
-(* TODO: Export to other languages: OCaml, Haskell *)
+(* TODO: Export to other languages: Haskell *)
 code_printing constant safe_sblit' \<rightharpoonup>
   (SML) "(fn/ ()/ => /array'_sblit _ _ _ _)"
   and (Scala) "{ ('_: Unit)/=>/
@@ -211,7 +241,13 @@ code_printing constant safe_sblit' \<rightharpoonup>
       safescopy(_.array,_.toInt,_.toInt,_.toInt)
     }"
 
-export_code safe_sblit checking SML Scala
+code_printing constant safe_sblit' \<rightharpoonup>
+ (OCaml) "(fun () -> /array'_sblit _ _ _ _)"
+
+
+export_code safe_sblit checking SML Scala OCaml
+
+
 
 
 subsection "Derived operations"
