thys/BTree/BTree_Map.thy
@@ -1,0 +1,91 @@
+theory BTree_Map
+imports BTree_Set "HOL-Data_Structures.Map_Specs"
+begin
+
+term "(1,2)"
+term int
+
+fun eq_kv where
+"eq_kv (k1, v1) (k2,v2) = (k1 = k2)"
+
+datatype ('a, 'b) ukv = KV 'a 'b
+
+quotient_type ('a,'b) kv  =  "('a, 'b) prod" / eq_kv
+  apply(rule equivpI)
+    apply (auto simp add: reflp_def symp_def transp_def)
+  done
+
+type_notation (ASCII)
+  kv  (infixr "\<mapsto>" 20)
+
+instantiation  kv :: (linorder, type) linorder
+begin
+
+fun less_eq_ukv::"'a \<times> 'b \<Rightarrow> 'a \<times> 'b \<Rightarrow> bool"
+  where "less_eq_ukv (k1, v1) (k2, v2) = (k1 \<le> k2)"
+
+lift_definition less_eq_kv :: "'a \<mapsto> 'b \<Rightarrow> 'a \<mapsto> 'b \<Rightarrow> bool" is less_eq_ukv
+  by auto
+
+definition less_kv:: "'a \<mapsto> 'b \<Rightarrow> 'a \<mapsto> 'b \<Rightarrow> bool"
+  where "less_kv a b = (a \<le> b \<and> \<not>b \<le> a)"
+
+
+instance
+proof(standard, goal_cases)
+  case (1 x y)
+  then show ?case by (simp add: less_kv_def)
+next
+  case (2 x)
+  then show ?case
+    by (transfer; clarsimp)
+next
+  case (3 x y z)
+  then show ?case
+    by (transfer; auto)
+next
+  case (4 x y)
+  then show ?case
+    by (transfer; auto)
+next
+  case (5 x y)
+  then show ?case
+    by (transfer; auto)
+qed
+end
+
+locale split_default = abs_split: BTree_Set.split split
+  for split::
+    "(('a \<mapsto> 'b) btree \<times> ('a::{linorder} \<mapsto> 'b::{default})) list \<Rightarrow> ('a \<mapsto> 'b)
+       \<Rightarrow> (('a \<mapsto> 'b) btree \<times> ('a \<mapsto> 'b)) list \<times> (('a \<mapsto> 'b) btree \<times> ('a \<mapsto> 'b)) list"
+begin
+
+lift_definition lift :: "'a \<Rightarrow> ('a \<mapsto> 'b)" is
+  "\<lambda>a. (a, default)" .
+
+lift_definition val :: "('a \<mapsto> 'b) \<Rightarrow> 'b" is
+  "\<lambda>(a,b). b"
+  apply auto
+  sorry
+
+fun find  where
+  "find (Leaf) y = None" |
+  "find (Node ts t) y = (
+      case split ts y of (_,(sub,sep)#rs) \<Rightarrow> (
+          if y = sep then
+             Some sep
+          else
+             find sub y
+      )
+   | (_,[]) \<Rightarrow> find t y
+  )"
+
+
+fun lookup :: "('a \<mapsto> 'b option) btree \<Rightarrow> 'a \<Rightarrow> 'a option"
+  where "lookup t x = (case find t (x,None) of Some (a,b) \<Rightarrow> Some b | None \<Rightarrow> None)"
+
+interpretation btree_map: Map_by_Ordered
+empty_btree 
+
+end
+end
