thys/BTree/README.md
@@ -27,11 +27,11 @@ All above mentioned files contain definitions as well as proofs of functional co
 
 ## Usage
 
-These theories have been tested with [Isabelle2020](https://isabelle.in.tum.de/website-Isabelle2020/index.html), although it should be compatible to newer versions of the tool.
+These theories have been tested with [Isabelle2021](https://isabelle.in.tum.de/website-Isabelle2021/index.html).
 
-The files `BTree*.thy` that do not contain `Imp` only need a regular Isabelle2020 setup.
+The files `BTree*.thy` that do not contain `Imp` only need a regular Isabelle setup.
 
-The rest of the theories build upon [Refine_Imperative_HOL](https://www.isa-afp.org/entries/Refine_Imperative_HOL.html), you will need to succesfully set up that project first as described in the [rArchive of Formal Proofs](https://www.isa-afp.org/using.html).
+The rest of the theories build upon [Refine_Imperative_HOL](https://www.isa-afp.org/entries/Refine_Imperative_HOL.html), you will need to succesfully set up that project first as described in the [Archive of Formal Proofs](https://www.isa-afp.org/using.html).
 The script `start_isabelle.sh` uses and if not available compiles a session
 containing the content of the Refinement Framework which significantly enhances
 working with the files provided in this project.
